theories/interop/update_laws.v
@@ -11,9 +11,9 @@ Section UpdateLaws.
 
 Context {hlc : has_lc}.
 Context {Σ : gFunctors}.
-Context `{!heapGS_ML Σ, !heapGS_C Σ}.
-Context `{!invGS_gen hlc Σ}.
-Context `{!wrapperGCtokGS Σ}.
+Context `{!heapG_ML Σ, !heapG_C Σ}.
+Context `{!invG Σ}.
+Context `{!wrapperGCtokG Σ}.
 
 Lemma ml_to_mut θ ℓ vs :
   ⊢ GC θ ∗ ℓ ↦∗ vs ==∗
