theories/interop/wp_ext_call_laws.v
@@ -18,9 +18,9 @@ Section Laws.
 
 Context {hlc : has_lc}.
 Context {Σ : gFunctors}.
-Context `{!heapGS_ML Σ, !heapGS_C Σ}.
-Context `{!invGS_gen hlc Σ}.
-Context `{!wrapperGS Σ}.
+Context `{!heapG_ML Σ, !heapG_C Σ}.
+Context `{!invG Σ}.
+Context `{!wrapperG Σ}.
 
 Notation MLval := ML_lang.val.
 Notation Cval := C_intf.val.
